Common/CBase.v
@@ -1,0 +1,46 @@
+
+From stdpp Require Export base.
+Require Import DecidableClass.
+Require Import Ensembles.
+
+
+(********** Notations **********)
+
+
+(** Functional pipe notation.
+
+    TODO figure out a correct parsing level. Currently is just below relation so
+    that a = b |> f will be parsed as a = (b |> f). *)
+Notation "v |> f" := (f v) (at level 69, only parsing, left associativity).
+
+
+(********* Utility functions **********)
+
+(** Convenient iff destruction *)
+Definition iffLR {A B : Prop} (i : A <-> B) : A -> B := proj1 i.
+Definition iffRL {A B : Prop} (i : A <-> B) : B -> A := proj2 i.
+
+(********** Constrained quantifiers **********)
+
+Global Instance Ensembles_elem_of {A} : ElemOf A (Ensemble A) := fun x P => P x.
+
+Definition forall_elem_of `{ElemOf A B} (P : A -> Prop) (b : B) :=
+  forall x : A, x ∈ b -> P x.
+
+Notation "∀' x ∈ b , P" := (forall_elem_of (fun x => P) b)
+  (at level 200, x binder, right associativity,
+  format "'[ ' '[ ' ∀' x  ∈  b ']' ,  '/' P ']'") : type_scope.
+
+Definition exists_elem_of `{ElemOf A B} (P : A -> Prop) (b : B) :=
+  exists x : A, x ∈ b /\ P x.
+
+Notation "∃' x ∈ b , P" := (exists_elem_of (fun x => P) b)
+  (at level 200, x binder, right associativity,
+  format "'[ ' '[ ' ∃' x  ∈  b ']' ,  '/' P ']'") : type_scope.
+
+Tactic Notation "unfold_cqual" :=
+  repeat unfold forall_elem_of in *;
+  repeat unfold exists_elem_of in *.
+
+Global Hint Unfold forall_elem_of : cqual.
+Global Hint Unfold exists_elem_of : cqual.
