Common/CBool.v
@@ -1,0 +1,73 @@
+(** This module cover all thing related to uses of boolean, mainly as decidable
+    proposition.
+
+    In particular it will cover boolean reflection and decidable generic
+    operations like equality. *)
+From stdpp Require Import base.
+From stdpp Require Export decidable.
+From Hammer Require Import Tactics.
+Require Export DecidableClass.
+
+Require Import CBase.
+
+(********** Boolean reflection **********)
+
+(* This is a hack to make CoqHammer boolean reflection use the Is_true coercion
+    from stdpp*)
+
+(* Using a plain Require and not Require Import is critical to not import the
+   is_true coercion since stdpp already uses the Is_true coercion.
+
+   TODO: In Coq 8.15 replace by Require Import -(coercion) Reflect. *)
+From Hammer Require Reflect.
+
+(** The breflect tactic copy-pasted from Hammer.Reflect because it cannot be *)
+(*     imported without coercion conflict prior to Coq 8.15 *)
+Tactic Notation "breflect" :=
+  try rewrite_strat topdown hints brefl.
+
+Tactic Notation "breflect" "in" hyp(H) :=
+  try rewrite_strat topdown hints brefl in H.
+
+Tactic Notation "breflect" "in" "*" :=
+  breflect;
+  repeat match goal with
+         | [H : _ |- _ ] => rewrite_strat topdown hints brefl in H
+         end.
+
+
+(* Convert the stdpp Is_True coercion to the is_true one that CoqHammer
+expects. *)
+Lemma true_is_true (b : bool) : b <-> is_true b.
+  Proof. sauto lq:on. Qed.
+#[global] Hint Rewrite -> true_is_true : brefl.
+#[global] Hint Rewrite <- true_is_true : breif.
+
+(* Unfortunately all boolean reflection lemmas will thus need be written with
+   is_true instead of the default coercion Is_True for now. When this project
+   start using Coq 8.15, this might change *)
+
+(********** Decidable propositions **********)
+
+(** Decidable equality notation that use the Decision type class from stdpp*)
+Notation "x =? y" := (bool_decide (x = y)) (at level 70, no associativity)
+    : stdpp_scope.
+
+(** Boolean reflection of decidable equality. *)
+Lemma bool_decide_is_true (P : Prop) {dec : Decision P} :
+  is_true (bool_decide P) <-> P.
+Proof. unfold is_true. apply bool_decide_eq_true. Qed.
+#[global] Hint Rewrite bool_decide_is_true : brefl.
+
+(** Convert automatical a Decidable instance (Coq standard library) to
+    a Decision instance (stdpp)
+
+    TODO: Decide (no pun intended) if we actually want to use Decidable or
+    Decision in this development. *)
+Global Instance Decidable_to_Decision P `{dec : Decidable P} : Decision P :=
+  match dec with
+  | {| Decidable_witness := true; Decidable_spec := spec |} =>
+   left ((iffLR spec) eq_refl)
+  | {| Decidable_witness := false; Decidable_spec := spec |} =>
+   right (fun HP => match (iffRL spec HP) with end)
+  end.
