Common/CList.v
@@ -1,0 +1,69 @@
+Require Import CBase CBool.
+From stdpp Require Import base.
+From stdpp Require Export list.
+
+(********** List automation **********)
+
+(** Automation for list simplifications *)
+Tactic Notation "list_simp" "in" "|-*" :=
+  rewrite_strat topdown hints list.
+
+Tactic Notation "list_simp" "in" hyp(H) :=
+  rewrite_strat topdown hints list in H.
+
+Tactic Notation "list_simp" :=
+  progress (try list_simp in |-*;
+  repeat match goal with
+         | [H : _ |- _ ] => rewrite_strat topdown hints list in H
+         end).
+
+Lemma elem_of_app {A} (l l' : list A) (a : A) :
+  a ∈ l ++ l' <-> a ∈ l \/ a ∈ l'.
+Proof. repeat rewrite elem_of_list_In. apply in_app_iff. Qed.
+#[global] Hint Rewrite @elem_of_app : list.
+
+(** Simple type class instance should be systematically simplfied *)
+Arguments list_subseteq _ _ _ /.
+
+Lemma Forall_forall_elem_of {A} (P : A -> Prop) (l : list A) :
+    Forall P l <-> ∀' x ∈ l, P x.
+Proof.
+  rewrite Forall_forall.
+  unfold forall_elem_of.
+  setoid_rewrite elem_of_list_In.
+  reflexivity.
+Qed.
+#[global] Hint Rewrite @Forall_forall_elem_of : list.
+
+Lemma elem_of_map {A B} (f : A → B) (l : list A) (x : A):
+  x ∈ l → (f x) ∈ (map f l).
+Proof. setoid_rewrite elem_of_list_In. apply in_map. Qed.
+#[global] Hint Resolve elem_of_map : list.
+
+
+
+(********** List boolean reflection **********)
+
+(** existsb boolean reflection *)
+Lemma existsb_brefl A (f : A → bool) (l : list A):
+  is_true (existsb f l) ↔ ∃' x ∈ l, is_true(f x).
+Proof.
+  unfold is_true.
+  rewrite existsb_exists.
+  unfold exists_elem_of.
+  setoid_rewrite elem_of_list_In.
+  reflexivity.
+Qed.
+#[global] Hint Rewrite existsb_brefl : brefl.
+
+(** forallb boolean reflection *)
+Lemma forallb_brefl A (f : A → bool) (l : list A):
+  is_true (forallb f l) ↔ ∀' x ∈ l, is_true(f x).
+Proof.
+  unfold is_true.
+  rewrite forallb_forall.
+  unfold forall_elem_of.
+  setoid_rewrite elem_of_list_In.
+  reflexivity.
+Qed.
+#[global] Hint Rewrite forallb_brefl : brefl.
