Common/Common.v
@@ -1,0 +1,29 @@
+(** This file is the top level of the SSCCommon library. Users should just
+    Require Import SSCCommon.Common.
+ *)
+
+From Hammer Require Export Tactics.
+From RecordUpdate Require Export RecordSet.
+Require Export bbv.Word.
+Require Import DecidableClass.
+From stdpp Require Export strings.
+
+Require Export CBase.
+Require Export CBool.
+Require Export CList.
+
+(********** Bitvectors **********)
+
+(* Interface Equality decision for words (from bbv) *)
+Global Instance word_eq_dec n : EqDecision (word n).
+Proof.
+  unfold EqDecision.
+  unfold Decision.
+  apply weq.
+Defined.
+
+(********** Utility functions **********)
+
+(** Update a function at a specific value *)
+Definition fun_add {A B} {_: EqDecision A} (k : A) (v : B) (f : A -> B) :=
+  fun x : A => if k =? x then v else f x.
